try to implement with indexed types

fstar/MemoryModel.fst
@@ -12,28 +12,26 @@ noeq type state_t = {
      bytemap: Map.t U16.t U8.t;
   }
 
-
-
-assume val r0: P.preorder state_t
-assume val r1: P.preorder state_t
+noeq type config = {
+     r0: P.preorder state_t;
+     r1: P.preorder state_t;
+  }
 
 let state_prop = state_t -> prop
 
 // pre-condition for write the value `v` at the index `k`
-let write_pre0 (k:U16.t) (v:U8.t) (p0:state_prop) : prop =
-  forall s. p0 s ==> r0 s {bytemap = Map.upd s.bytemap k v}
+let write_pre0 (c:config) (k:U16.t) (v:U8.t) (p0:state_prop) : prop =
+  forall s. p0 s ==> c.r0 s {bytemap = Map.upd s.bytemap k v}
 
-let write_post0 (k:U16.t) (v:U8.t) (p0:state_prop) (p1:state_prop) : prop =
-  forall y. p1 y <==> (exists x.
-    p0 x /\ r1 {bytemap = Map.upd x.bytemap k v} y
-  )
+let write_post0 (c:config) (k:U16.t) (v:U8.t) (p0:state_prop) (y:state_t) : prop = 
+  exists x. p0 x /\ c.r1 {bytemap = Map.upd x.bytemap k v} y
 
-let read_post0 (k:U16.t) (p0:state_prop) (v:U8.t) (p1:state_prop) : prop =
-  let p (s:state_t) =
-    p0 s /\ Map.sel s.bytemap k == v
-  in (exists s. p s) /\ (forall y. p1 y <==> (
-    exists x. p x /\ r1 x y
-  ))
+
+let read_post0 (c:config) (k:U16.t) (p0:state_prop) (v:U8.t) (y:state_t) : prop =
+  exists x. p0 x /\ Map.sel x.bytemap k == v /\ c.r1 x y
+
+let read_post0' (c:config) (k:U16.t) (p0:state_prop) (v:U8.t) : prop =
+  exists s. p0 s /\ Map.sel s.bytemap k == v
 
 new_effect NONDET_STATE = STATE_h state_prop
 
@@ -42,33 +40,70 @@ unfold let lift_div_state (a:Type) (wp:pure_wp a) (p:a -> state_prop -> Type0) (
 
 sub_effect DIV ~> NONDET_STATE = lift_div_state
 
-effect ST (a:Type)
+effect ST (a:Type) (c:config)
   (pre:state_prop -> Type0)
   (post: (h:state_prop -> a -> _:state_prop{pre h} -> Type0)) =
   NONDET_STATE a (fun (p:(a -> state_prop -> Type0)) (h:state_prop) ->
     pre h /\ (forall a h1. post h a h1 ==> p a h1))
 
-effect St (a:Type) = ST a (fun h -> True) (fun h0 r h1 -> True)
+effect St (a:Type) (c:config) = ST a c (fun h -> True) (fun h0 r h1 -> True)
 
-assume val read0 (k:U16.t) :
-  ST U8.t
+assume val read0 (#c:config) (k:U16.t) :
+  ST U8.t c
     (fun p0 -> True)
-    (read_post0 k)
+    (fun p0 v p1 -> read_post0' c k p0 v /\ p1 == read_post0 c k p0 v)
 
-assume val write0 (k:U16.t) (v:U8.t) :
-  ST unit
-    (write_pre0 k v)
-    (fun p0 _ -> write_post0 k v p0)
+assume val write0 (#c:config) (k:U16.t) (v:U8.t) :
+  ST unit c
+    (write_pre0 c k v)
+    (fun p0 _ p1 -> p1 == write_post0 c k v p0)
 
 
-assume val cas0 (key:U16.t) (old_v new_v:U8.t) :
-  ST (option U8.t)
+assume val cas0 (#c:config) (key:U16.t) (old_v new_v:U8.t) :
+  ST (option U8.t) c
     (fun p0 -> True)
     (fun p0 r p1 ->
       (None? r ==>
-        write_pre0 key new_v (fun s -> p0 s /\ Map.sel s.bytemap key == old_v) /\
-        write_post0 key new_v (fun s -> p0 s /\ Map.sel s.bytemap key == old_v) p1
+        write_pre0 c key new_v (fun s -> p0 s /\ Map.sel s.bytemap key == old_v) /\
+        p1 == write_post0 c key new_v (fun s -> p0 s /\ Map.sel s.bytemap key == old_v)
       ) /\ (Some? r ==> (r <> Some old_v /\
-        read_post0 key p0 (match r with | Some x -> x) p1
+        p1 == read_post0 c key p0 (match r with | Some x -> x) /\
+        read_post0' c key p0 (match r with | Some x -> x)
       ))
     )
+
+let c0 = {
+    r0 = (fun s1 s2 -> s1 == s2 \/
+      ((
+        Map.sel s1.bytemap 0us == 0uy \/
+        Map.sel s1.bytemap 0us == 1uy
+      ) /\ (
+        Map.sel s2.bytemap 0us == 0uy \/
+        Map.sel s2.bytemap 0us == 1uy
+      )
+    ));
+    r1 = (fun s1 s2 -> s1 == s2 \/ (
+      (
+        Map.sel s1.bytemap 0us == 0uy \/
+        Map.sel s1.bytemap 0us == 2uy
+      ) /\ (
+        Map.sel s1.bytemap 0us == 0uy \/
+        Map.sel s2.bytemap 0us == 2uy
+      )
+    ))
+  }
+
+let c1 = {
+    r1 = c0.r0;
+    r0 = c0.r1
+  }
+
+#push-options "--z3rlimit 50"
+let prog0 (_:unit) :
+  St unit c0 =
+  match cas0 #c0 0us 0uy 1uy with
+  | Some v -> ()
+  | None ->
+    write0 #c0 1us 42uy;
+    write0 #c0 2us 43uy;
+    write0 #c0 0us 0uy
